src/lowparse/LowParse.SteelST.SeqMatch.fst
@@ -1,0 +1,1163 @@
+module LowParse.SteelST.SeqMatch
+include LowParse.SteelST.VCList
+open Steel.ST.OnRange
+open Steel.ST.GenElim
+
+module Seq = FStar.Seq
+module R = Steel.ST.Reference
+module A = Steel.ST.Array
+module AP = LowParse.SteelST.ArrayPtr
+module SZ = FStar.SizeT
+
+(* `seq_list_match` describes how to match a sequence of low-level
+values (the low-level contents of an array) with a list of high-level
+values. `seq_list_match` is carefully designed to be usable within
+(mutually) recursive definitions of matching functions on the type of
+high-level values.  *)
+
+[@@__reduce__]
+let seq_list_match_nil0
+  (#t: Type0) // FIXME: universe polymorphism may be a problem with Steel
+  (c: Seq.seq t)
+: Tot vprop
+= pure (c `Seq.equal` Seq.empty)
+
+[@@__reduce__]
+let seq_list_match_cons0
+  (#t #t': Type0) // FIXME: universe polymorphism may be a problem with Steel
+  (c: Seq.seq t)
+  (l: list t' { Cons? l })
+  (item_match: (t -> (v': t' { v' << l }) -> vprop))
+  (seq_list_match: (Seq.seq t -> (v': list t') -> (raw_data_item_match: (t -> (v'': t' { v'' << v' }) -> vprop) { v' << l }) ->
+vprop))
+: Tot vprop
+= exists_ (fun (c1: t) -> exists_ (fun (c2: Seq.seq t) ->
+    item_match c1 (List.Tot.hd l) `star`
+    seq_list_match c2 (List.Tot.tl l) item_match `star`
+    pure (c `Seq.equal` Seq.cons c1 c2)
+  ))
+
+let rec seq_list_match
+  (#t #t': Type)
+  (c: Seq.seq t)
+  (v: list t')
+  (item_match: (t -> (v': t' { v' << v }) -> vprop))
+: Tot vprop
+  (decreases v)
+= if Nil? v
+  then seq_list_match_nil0 c
+  else seq_list_match_cons0 c v item_match seq_list_match
+
+let seq_list_match_cons_eq
+  (#t #t': Type)
+  (c: Seq.seq t)
+  (v: list t')
+  (item_match: (t -> (v': t' { v' << v }) -> vprop))
+: Lemma
+  (requires (Cons? v))
+  (ensures (
+    seq_list_match c v item_match ==
+    seq_list_match_cons0 c v item_match seq_list_match
+  ))
+= let a :: q = v in
+  assert_norm (seq_list_match c (a :: q) item_match ==
+    seq_list_match_cons0 c (a :: q) item_match seq_list_match
+  )
+
+(* `seq_seq_match` describes how to match a sequence of low-level
+values (the low-level contents of an array) with a sequence of high-level
+values. Contrary to `seq_list_match`, `seq_seq_match` is not meant to be usable within
+(mutually) recursive definitions of matching functions on the type of
+high-level values, because no lemma ensures that `Seq.index s i << s`  *)
+
+let seq_seq_match_item
+  (#t1 #t2: Type0) // FIXME: universe polymorphism may be a problem with Steel
+  (p: t1 -> t2 -> vprop)
+  (c: Seq.seq t1)
+  (l: Seq.seq t2)
+  (i: nat)
+: Tot vprop
+= if i < Seq.length c && i < Seq.length l
+  then
+    p (Seq.index c i) (Seq.index l i)
+  else
+    pure (squash False)
+
+let seq_seq_match_item_tail
+  (#t1 #t2: Type)
+  (p: t1 -> t2 -> vprop)
+  (c: Seq.seq t1)
+  (l: Seq.seq t2)
+  (delta: nat)
+  (i: nat)
+: Lemma
+  (requires (
+    i + delta <= Seq.length c /\
+    i + delta <= Seq.length l
+  ))
+  (ensures (
+    seq_seq_match_item p (Seq.slice c delta (Seq.length c)) (Seq.slice l delta (Seq.length l)) i ==
+      seq_seq_match_item p c l (i + delta)
+  ))
+= ()
+
+[@@__reduce__]
+let seq_seq_match
+  (#t1 #t2: Type)
+  (p: t1 -> t2 -> vprop)
+  (c: Seq.seq t1)
+  (l: Seq.seq t2)
+  (i j: nat)
+: Tot vprop
+= on_range (seq_seq_match_item p c l) i j
+
+let seq_seq_match_length
+  (#opened: _)
+  (#t1 #t2: Type)
+  (p: t1 -> t2 -> vprop)
+  (s1: Seq.seq t1)
+  (s2: Seq.seq t2)
+  (i j: nat)
+: STGhost unit opened
+    (seq_seq_match p s1 s2 i j)
+    (fun _ -> seq_seq_match p s1 s2 i j)
+    True
+    (fun _ -> i <= j /\ (i == j \/ (j <= Seq.length s1 /\ j <= Seq.length s2)))
+= on_range_le (seq_seq_match_item p s1 s2) i j;
+  if i = j
+  then noop ()
+  else begin
+    let j' = j - 1 in
+    if j' < Seq.length s1 && j' < Seq.length s2
+    then noop ()
+    else begin
+      on_range_unsnoc
+        (seq_seq_match_item p s1 s2)
+        i j' j;
+      rewrite
+        (seq_seq_match_item p _ _ _)
+        (pure (squash False));
+      let _ = gen_elim () in
+      rewrite
+        (seq_seq_match p s1 s2 i j')
+        (seq_seq_match p s1 s2 i j) // by contradiction
+    end
+  end
+
+let seq_seq_match_weaken
+  (#opened: _)
+  (#t1 #t2: Type)
+  (p p': t1 -> t2 -> vprop)
+  (w: ((x1: t1) -> (x2: t2) -> STGhostT unit opened
+    (p x1 x2) (fun _ -> p' x1 x2)
+  ))
+  (c1 c1': Seq.seq t1)
+  (c2 c2': Seq.seq t2)
+  (i j: nat)
+: STGhost unit opened
+    (seq_seq_match p c1 c2 i j)
+    (fun _ -> seq_seq_match p' c1' c2' i j)
+    (i <= j /\ (i == j \/ (
+      j <= Seq.length c1 /\ j <= Seq.length c2 /\
+      j <= Seq.length c1' /\ j <= Seq.length c2' /\
+      Seq.slice c1 i j `Seq.equal` Seq.slice c1' i j /\
+      Seq.slice c2 i j `Seq.equal` Seq.slice c2' i j
+    )))
+    (fun _ -> True)
+=
+  on_range_weaken
+    (seq_seq_match_item p c1 c2)
+    (seq_seq_match_item p' c1' c2')
+    i j
+    (fun k ->
+       rewrite (seq_seq_match_item p c1 c2 k) (p (Seq.index (Seq.slice c1 i j) (k - i)) (Seq.index (Seq.slice c2 i j) (k - i)));
+       w _ _;
+       rewrite (p' _ _) (seq_seq_match_item p' c1' c2' k)
+    )
+
+let seq_seq_match_weaken_with_implies
+  (#opened: _)
+  (#t1 #t2: Type)
+  (p: t1 -> t2 -> vprop)
+  (c1 c1': Seq.seq t1)
+  (c2 c2': Seq.seq t2)
+  (i j: nat)
+: STGhost unit opened
+    (seq_seq_match p c1 c2 i j)
+    (fun _ -> seq_seq_match p c1' c2' i j `star`
+      (seq_seq_match p c1' c2' i j `implies_` seq_seq_match p c1 c2 i j)
+    )
+    (i <= j /\ (i == j \/ (
+      j <= Seq.length c1 /\ j <= Seq.length c2 /\
+      j <= Seq.length c1' /\ j <= Seq.length c2' /\
+      Seq.slice c1 i j `Seq.equal` Seq.slice c1' i j /\
+      Seq.slice c2 i j `Seq.equal` Seq.slice c2' i j
+    )))
+    (fun _ -> True)
+= seq_seq_match_weaken
+    p p (fun _ _ -> noop ())
+    c1 c1'
+    c2 c2'
+    i j;
+  intro_implies
+    (seq_seq_match p c1' c2' i j)
+    (seq_seq_match p c1 c2 i j)
+    emp
+    (fun _ ->
+      seq_seq_match_weaken
+        p p (fun _ _ -> noop ())
+        c1' c1
+        c2' c2
+        i j
+    )
+
+(* Going between `seq_list_match` and `seq_seq_match` *)
+
+let rec list_index_append_cons
+  (#t: Type)
+  (l1: list t)
+  (a: t)
+  (l2: list t)
+: Lemma
+  (ensures (let l = l1 `List.Tot.append` (a :: l2) in
+    let n1 = List.Tot.length l1 in
+    n1 < List.Tot.length l /\
+    List.Tot.index l n1 == a
+  ))
+  (decreases l1)
+= match l1 with
+  | [] -> ()
+  | a1 :: l1' -> list_index_append_cons l1' a l2
+
+let rec list_index_map
+  (#t1 #t2: Type)
+  (f: (t1 -> t2))
+  (l1: list t1)
+  (i: nat {i < List.Tot.length l1})
+: Lemma
+  (ensures (let l2 = List.Tot.map f l1 in
+    List.Tot.length l1 == List.Tot.length l2 /\
+    List.Tot.index l2 i == f (List.Tot.index l1 i)
+  ))
+  [SMTPat (List.Tot.index (List.Tot.map f l1) i)]
+= let a :: l1' = l1 in
+  if i = 0
+  then ()
+  else list_index_map f l1' (i - 1)
+
+let seq_of_list_eq_init_index
+  (#t: Type)
+  (l: list t)
+: Lemma
+  (Seq.seq_of_list l `Seq.equal` Seq.init (List.Tot.length l) (List.Tot.index l))
+= () // thanks to Seq.lemma_seq_of_list_index
+
+let seq_of_list_tail
+  (#t: Type)
+  (a: t)
+  (q: list t)
+: Lemma
+  (Seq.tail (Seq.seq_of_list (a :: q)) == Seq.seq_of_list q)
+= Seq.lemma_seq_of_list_induction (a :: q)
+
+
+let seq_seq_match_tail_elim
+  (#t1 #t2: Type)
+  (#opened: _)
+  (p: t1 -> t2 -> vprop)
+  (c: Seq.seq t1)
+  (l: Seq.seq (t2))
+  (delta: nat {
+    delta <= Seq.length c /\
+    delta <= Seq.length l
+  })
+  (i j: nat)
+: STGhostT unit opened
+    (seq_seq_match p (Seq.slice c delta (Seq.length c)) (Seq.slice l delta (Seq.length l)) i j)
+    (fun _ -> seq_seq_match p c l (i + delta) (j + delta))
+= on_range_le (seq_seq_match_item p _ _) _ _;
+  on_range_weaken_and_shift
+    (seq_seq_match_item p (Seq.slice c delta (Seq.length c)) (Seq.slice l delta (Seq.length l)))
+    (seq_seq_match_item p c l)
+    delta
+    i j
+    (fun k ->
+       if k < Seq.length c - delta && k < Seq.length l - delta
+       then begin
+         seq_seq_match_item_tail p c l delta k;
+         rewrite
+           (seq_seq_match_item p (Seq.slice c delta (Seq.length c)) (Seq.slice l delta (Seq.length l)) k)
+           (seq_seq_match_item p c l (k + delta))
+       end else begin
+         rewrite
+           (seq_seq_match_item p (Seq.slice c delta (Seq.length c)) (Seq.slice l delta (Seq.length l)) k)
+           (pure (squash False));
+         let _ = gen_elim () in
+         rewrite
+           emp
+           (seq_seq_match_item p c l (k + delta)) // by contradiction
+       end
+    )
+    (i + delta) (j + delta)
+
+let seq_seq_match_tail_intro
+  (#t1 #t2: Type)
+  (#opened: _)
+  (p: t1 -> t2 -> vprop)
+  (c: Seq.seq t1)
+  (l: Seq.seq t2)
+  (delta: nat {
+    delta <= Seq.length c /\
+    delta <= Seq.length l
+  })
+  (i: nat {
+    delta <= i
+  })
+  (j: nat)
+: STGhostT (squash (i <= j)) opened
+    (seq_seq_match p c l i j)
+    (fun _ -> seq_seq_match p (Seq.slice c delta (Seq.length c)) (Seq.slice l delta (Seq.length l)) (i - delta) (j - delta))
+= on_range_le (seq_seq_match_item p _ _) _ _;
+  on_range_weaken_and_shift
+    (seq_seq_match_item p c l)
+    (seq_seq_match_item p (Seq.slice c delta (Seq.length c)) (Seq.slice l delta (Seq.length l)))
+    (0 - delta)
+    i j
+    (fun k ->
+      if k < Seq.length c && k < Seq.length l
+      then begin
+        seq_seq_match_item_tail p c l delta (k - delta);
+        rewrite
+          (seq_seq_match_item p c l k)
+          (seq_seq_match_item p (Seq.slice c delta (Seq.length c)) (Seq.slice l delta (Seq.length l)) (k + (0 - delta)))
+      end else begin
+        rewrite
+          (seq_seq_match_item p c l k)
+          (pure (squash False));
+        let _ = gen_elim () in
+        rewrite
+          emp
+          (seq_seq_match_item p (Seq.slice c delta (Seq.length c)) (Seq.slice l delta (Seq.length l)) (k + (0 - delta))) // by contradiction
+      end
+    )
+    (i - delta) (j - delta)
+
+let rec seq_seq_match_seq_list_match
+  (#opened: _)
+  (#t1 #t2: Type)
+  (p: t1 -> t2 -> vprop)
+  (c: Seq.seq t1)
+  (l: list t2)
+: STGhost unit opened
+    (seq_seq_match p c (Seq.seq_of_list l) 0 (List.Tot.length l))
+    (fun _ -> seq_list_match c l p)
+    (Seq.length c == List.Tot.length l)
+    (fun _ -> True)
+    (decreases l)
+= match l with
+  | [] ->
+    drop (seq_seq_match p _ _ _ _);
+    rewrite
+      (seq_list_match_nil0 c)
+      (seq_list_match c l p)
+  | a :: q ->
+    Seq.lemma_seq_of_list_induction (a :: q);
+    seq_list_match_cons_eq c l p;
+    on_range_uncons
+      (seq_seq_match_item p _ _)
+      _ 1 _;
+    rewrite
+      (seq_seq_match_item p _ _ _)
+      (p (Seq.head c) (List.Tot.hd l));
+    let _ = seq_seq_match_tail_intro
+      p _ _ 1 _ _
+    in
+    rewrite
+      (seq_seq_match p _ _ _ _)
+      (seq_seq_match p (Seq.tail c) (Seq.seq_of_list (List.Tot.tl l)) 0 (List.Tot.length (List.Tot.tl l)));
+    seq_seq_match_seq_list_match p _ (List.Tot.tl l);
+    rewrite
+      (seq_list_match_cons0 c l p seq_list_match)
+      (seq_list_match c l p)
+
+let rec seq_list_match_seq_seq_match
+  (#opened: _)
+  (#t1 #t2: Type)
+  (p: t1 -> t2 -> vprop)
+  (c: Seq.seq t1)
+  (l: list t2)
+: STGhost unit opened
+    (seq_list_match c l p)
+    (fun _ -> seq_seq_match p c (Seq.seq_of_list l) 0 (List.Tot.length l))
+    True
+    (fun _ -> Seq.length c == List.Tot.length l)
+    (decreases l)
+= match l with
+  | [] ->
+    rewrite
+      (seq_list_match c l p)
+      (seq_list_match_nil0 c);
+    let _ = gen_elim () in
+    on_range_empty
+      (seq_seq_match_item p c (Seq.seq_of_list l))
+      0
+      (List.Tot.length l)
+  | a :: q ->
+    let _l_nonempty : squash (Cons? l) = () in
+    Seq.lemma_seq_of_list_induction (a :: q);
+    seq_list_match_cons_eq c l p;
+    noop ();
+    rewrite
+      (seq_list_match c l p)
+      (seq_list_match_cons0 c l p seq_list_match);
+    let _ = gen_elim () in
+    let a' = vpattern (fun a' -> p a' _) in
+    let c' = vpattern (fun c' -> seq_list_match c' _ _) in
+    Seq.lemma_cons_inj (Seq.head c) a' (Seq.tail c) c';
+    assert (a' == Seq.head c);
+    assert (c' == Seq.tail c);
+    noop ();
+    seq_list_match_seq_seq_match p _ _;
+    rewrite
+      (seq_seq_match p _ _ _ _)
+      (seq_seq_match p (Seq.slice c 1 (Seq.length c)) (Seq.slice (Seq.seq_of_list l) 1 (Seq.length (Seq.seq_of_list l))) 0 (List.Tot.length (List.Tot.tl l)));
+    let _ = seq_seq_match_tail_elim
+      p c (Seq.seq_of_list l) 1 0 (List.Tot.length (List.Tot.tl l))
+    in
+    rewrite
+      (seq_seq_match p _ _ _ _)
+      (seq_seq_match p c (Seq.seq_of_list l) 1 (List.Tot.length l));
+    rewrite
+      (p _ _)
+      (seq_seq_match_item p c (Seq.seq_of_list l) 0);
+    on_range_cons
+      (seq_seq_match_item p _ _)
+      0 1 (List.Tot.length l)
+
+let seq_seq_match_seq_list_match_with_implies
+  (#opened: _)
+  (#t1 #t2: Type)
+  (p: t1 -> t2 -> vprop)
+  (c: Seq.seq t1)
+  (l: list t2)
+: STGhost unit opened
+    (seq_seq_match p c (Seq.seq_of_list l) 0 (List.Tot.length l))
+    (fun _ -> seq_list_match c l p `star` (seq_list_match c l p `implies_` seq_seq_match p c (Seq.seq_of_list l) 0 (List.Tot.length l)))
+    (Seq.length c == List.Tot.length l)
+    (fun _ -> True)
+= seq_seq_match_seq_list_match p c l;
+  intro_implies
+    (seq_list_match c l p)
+    (seq_seq_match p c (Seq.seq_of_list l) 0 (List.Tot.length l))
+    emp
+    (fun _ -> seq_list_match_seq_seq_match p c l)
+
+let seq_list_match_seq_seq_match_with_implies
+  (#opened: _)
+  (#t1 #t2: Type)
+  (p: t1 -> t2 -> vprop)
+  (c: Seq.seq t1)
+  (l: list t2)
+: STGhost unit opened
+    (seq_list_match c l p)
+    (fun _ -> seq_seq_match p c (Seq.seq_of_list l) 0 (List.Tot.length l) `star` (seq_seq_match p c (Seq.seq_of_list l) 0 (List.Tot.length l) `implies_` seq_list_match c l p))
+    True
+    (fun _ -> Seq.length c == List.Tot.length l)
+= seq_list_match_seq_seq_match p c l;
+  intro_implies
+    (seq_seq_match p c (Seq.seq_of_list l) 0 (List.Tot.length l))
+    (seq_list_match c l p)
+    emp
+    (fun _ -> seq_seq_match_seq_list_match p c l)
+
+(* Random array access
+
+Since `seq_list_match` is defined recursively on the list of
+high-level values, it is used naturally left-to-right. By contrast,
+in practice, an application may populate an array in a different
+order, or even out-of-order. `seq_seq_match` supports that scenario
+better, as we show below.
+
+*)
+
+let seq_map (#t1 #t2: Type) (f: t1 -> t2) (s: Seq.seq t1) : Tot (Seq.seq t2) =
+  Seq.init (Seq.length s) (fun i -> f (Seq.index s i))
+
+let rec seq_map_seq_of_list (#t1 #t2: Type) (f: t1 -> t2) (l: list t1) : Lemma
+  (seq_map f (Seq.seq_of_list l) `Seq.equal` Seq.seq_of_list (List.Tot.map f l))
+= match l with
+  | [] -> ()
+  | a :: q -> seq_map_seq_of_list f q
+
+let item_match_option
+  (#t1 #t2: Type)
+  (p: t1 -> t2 -> vprop)
+  (x1: t1)
+  (x2: option t2)
+: Tot vprop
+= match x2 with
+  | None -> emp
+  | Some x2' -> p x1 x2'
+
+let seq_seq_match_item_match_option_elim
+  (#opened: _)
+  (#t1 #t2: Type)
+  (p: t1 -> t2 -> vprop)
+  (s1: Seq.seq t1)
+  (s2: Seq.seq t2)
+  (i j: nat)
+: STGhostT unit opened
+    (seq_seq_match (item_match_option p) s1 (seq_map Some s2) i j)
+    (fun _ -> seq_seq_match p s1 s2 i j)
+= on_range_weaken
+    (seq_seq_match_item (item_match_option p) s1 (seq_map Some s2))
+    (seq_seq_match_item p s1 s2)
+    i j
+    (fun k ->
+      rewrite
+        (seq_seq_match_item (item_match_option p) s1 (seq_map Some s2) k)
+        (seq_seq_match_item p s1 s2 k)
+    )
+
+let seq_seq_match_item_match_option_intro
+  (#opened: _)
+  (#t1 #t2: Type)
+  (p: t1 -> t2 -> vprop)
+  (s1: Seq.seq t1)
+  (s2: Seq.seq t2)
+  (i j: nat)
+: STGhostT unit opened
+    (seq_seq_match p s1 s2 i j)
+    (fun _ -> seq_seq_match (item_match_option p) s1 (seq_map Some s2) i j)
+= on_range_weaken
+    (seq_seq_match_item p s1 s2)
+    (seq_seq_match_item (item_match_option p) s1 (seq_map Some s2))
+    i j
+    (fun k ->
+      rewrite
+        (seq_seq_match_item p s1 s2 k)
+        (seq_seq_match_item (item_match_option p) s1 (seq_map Some s2) k)
+    )
+
+let rec seq_seq_match_item_match_option_init
+  (#opened: _)
+  (#t1 #t2: Type)
+  (p: t1 -> t2 -> vprop)
+  (s: Seq.seq t1)
+: STGhostT unit opened
+    emp
+    (fun _ -> seq_seq_match (item_match_option p) s (Seq.create (Seq.length s) None) 0 (Seq.length s))
+    (decreases (Seq.length s))
+= if Seq.length s = 0
+  then
+    on_range_empty (seq_seq_match_item (item_match_option p) s (Seq.create (Seq.length s) None)) 0 (Seq.length s)
+  else begin
+    seq_seq_match_item_match_option_init p (Seq.tail s);
+    on_range_weaken_and_shift
+      (seq_seq_match_item (item_match_option p) (Seq.tail s) (Seq.create (Seq.length (Seq.tail s)) None))
+      (seq_seq_match_item (item_match_option p) s (Seq.create (Seq.length s) None))
+      1
+      0
+      (Seq.length (Seq.tail s))
+      (fun k ->
+        rewrite
+          (seq_seq_match_item (item_match_option p) (Seq.tail s) (Seq.create (Seq.length (Seq.tail s)) None) k)
+          (seq_seq_match_item (item_match_option p) s (Seq.create (Seq.length s) None) (k + 1))
+      )
+      1
+      (Seq.length s);
+    rewrite
+      emp
+      (seq_seq_match_item (item_match_option p) s (Seq.create (Seq.length s) None) 0);
+    on_range_cons
+      (seq_seq_match_item (item_match_option p) s (Seq.create (Seq.length s) None))
+      0
+      1
+      (Seq.length s)
+  end
+
+let seq_seq_match_upd
+  (#opened: _)
+  (#t1 #t2: Type)
+  (p: t1 -> t2 -> vprop)
+  (s1: Seq.seq t1)
+  (s2: Seq.seq t2)
+  (i j: nat)
+  (k: nat {
+    i <= j /\ j < k
+  })
+  (x1: t1)
+  (x2: t2)
+: STGhostT (squash (j < Seq.length s1 /\ j < Seq.length s2)) opened
+    (seq_seq_match p s1 s2 i k `star` p x1 x2)
+    (fun _ -> 
+      seq_seq_match p (Seq.upd s1 j x1) (Seq.upd s2 j x2) i k
+    )
+= seq_seq_match_length p s1 s2 i k;
+  on_range_get
+    (seq_seq_match_item p s1 s2)
+    i j (j + 1) k;
+  let res : squash (j < Seq.length s1 /\ j < Seq.length s2) = () in
+  drop (seq_seq_match_item p s1 s2 j);
+  rewrite
+    (p x1 x2)
+    (seq_seq_match_item p (Seq.upd s1 j x1) (Seq.upd s2 j x2) j);
+  seq_seq_match_weaken
+    p p (fun _ _ -> noop ())
+    s1 (Seq.upd s1 j x1)
+    s2 (Seq.upd s2 j x2)
+    i j;
+  seq_seq_match_weaken
+    p p (fun _ _ -> noop ())
+    s1 (Seq.upd s1 j x1)
+    s2 (Seq.upd s2 j x2)
+    (j + 1) k;
+  on_range_put
+    (seq_seq_match_item p (Seq.upd s1 j x1) (Seq.upd s2 j x2))
+    i j j (j + 1) k;
+  res
+    
+let seq_seq_match_item_match_option_upd
+  (#opened: _)
+  (#t1 #t2: Type)
+  (p: t1 -> t2 -> vprop)
+  (s1: Seq.seq t1)
+  (s2: Seq.seq (option t2))
+  (i j: nat)
+  (k: nat {
+    i <= j /\ j < k
+  })
+  (x1: t1)
+  (x2: t2)
+: STGhostT (squash (j < Seq.length s1 /\ j < Seq.length s2)) opened
+    (seq_seq_match (item_match_option p) s1 s2 i k `star` p x1 x2)
+    (fun _ -> 
+      seq_seq_match (item_match_option p) (Seq.upd s1 j x1) (Seq.upd s2 j (Some x2)) i k
+    )
+= rewrite
+    (p x1 x2)
+    (item_match_option p x1 (Some x2));
+  seq_seq_match_upd (item_match_option p) s1 s2 i j k x1 (Some x2)
+
+let seq_seq_match_item_match_option_index
+  (#opened: _)
+  (#t1 #t2: Type)
+  (p: t1 -> t2 -> vprop)
+  (s1: Seq.seq t1)
+  (s2: Seq.seq (option t2))
+  (i j: nat)
+  (k: nat {
+    i <= j /\ j < k /\
+    (j < Seq.length s2 ==> Some? (Seq.index s2 j))
+  })
+: STGhostT (squash (j < Seq.length s1 /\ j < Seq.length s2 /\ Some? (Seq.index s2 j))) opened
+    (seq_seq_match (item_match_option p) s1 s2 i k)
+    (fun _ -> 
+      seq_seq_match (item_match_option p) s1 (Seq.upd s2 j None) i k `star`
+      p (Seq.index s1 j) (Some?.v (Seq.index s2 j))
+    )
+= seq_seq_match_length (item_match_option p) s1 s2 i k;
+  on_range_get
+    (seq_seq_match_item (item_match_option p) s1 s2)
+    i j (j + 1) k;
+  let res : squash (j < Seq.length s1 /\ j < Seq.length s2 /\ Some? (Seq.index s2 j)) = () in
+  rewrite
+    (seq_seq_match_item (item_match_option p) s1 s2 j)
+    (p (Seq.index s1 j) (Some?.v (Seq.index s2 j)));
+  rewrite
+    emp
+    (seq_seq_match_item (item_match_option p) s1 (Seq.upd s2 j None) j);
+  seq_seq_match_weaken
+    (item_match_option p) (item_match_option p) (fun _ _ -> noop ())
+    s1 s1
+    s2 (Seq.upd s2 j None)
+    i j;
+  seq_seq_match_weaken
+    (item_match_option p) (item_match_option p) (fun _ _ -> noop ())
+    s1 s1
+    s2 (Seq.upd s2 j None)
+    (j + 1) k;
+  on_range_put
+    (seq_seq_match_item (item_match_option p) s1 (Seq.upd s2 j None))
+    i j j (j + 1) k;
+  res
+
+(* Parsing into an array
+
+While this implementation also works if the low-level value type is a pointer type, the resulting C code may not be idiomatic. Also, it assumes that the parsing function for elements always succeeds (e.g. in the case of an array of pointers, `alloc` never returns NULL.)
+
+*)
+
+noextract
+unfold
+let read_array_payload_invariant_prop0
+  (#t: Type)
+  (#t': Type)
+  (k: parser_kind)
+  (n0: SZ.t)
+  (vl0: v parse_list_kind (list t'))
+  (cont: bool)
+  (s: Seq.seq t)
+  (l1: list t')
+  (vr: v parse_list_kind (list t'))
+  (n: SZ.t)
+  (n': nat)
+: Tot prop
+=
+      k.parser_kind_subkind == Some ParserStrong /\
+      SZ.v n0 == List.Tot.length vl0.contents /\
+      SZ.v n == List.Tot.length l1 /\
+      Seq.length s == SZ.v n0 /\
+      List.Tot.append l1 vr.contents == vl0.contents /\
+      n' == SZ.v n /\
+      (cont == true <==> (SZ.v n < SZ.v n0))
+
+noextract
+let read_array_payload_invariant_prop
+  (#t #t': Type)
+  (k: parser_kind)
+  (n0: SZ.t)
+  (vl0: v parse_list_kind (list t'))
+  (cont: bool)
+  (s: Seq.seq t)
+  (l1: list t')
+  (vr: v parse_list_kind (list t'))
+  (n: SZ.t)
+  (n': nat)
+: Tot prop
+= read_array_payload_invariant_prop0 k n0 vl0 cont s l1 vr n n'
+
+[@@__reduce__]
+let read_array_payload_invariant_body0
+  (#t #t': Type)
+  (#k: parser_kind)
+  (p: parser k t')
+  (item_match: t -> t' -> vprop)
+  (n0: SZ.t)
+  (vl0: v parse_list_kind (list t'))
+  (l0: byte_array)
+  (a0: A.array t)
+  (pn: R.ref SZ.t)
+  (pr: R.ref byte_array)
+  (s: Seq.seq t)
+  (l1: list t')
+  (r: byte_array)
+  (vr: v parse_list_kind (list t'))
+  (n: SZ.t)
+  (n': nat)
+: Tot vprop
+=
+    A.pts_to a0 full_perm s `star`
+    R.pts_to pn full_perm n `star`
+    R.pts_to pr full_perm r `star`
+    seq_seq_match item_match s (Seq.seq_of_list vl0.contents) 0 n' `star`
+    aparse (parse_list p) r vr `star`
+    ((seq_seq_match item_match s (Seq.seq_of_list vl0.contents) 0 n' `star` aparse (parse_list p) r vr) `implies_`
+      aparse (parse_list p) l0 vl0)
+
+[@@erasable]
+noeq
+type read_array_payload_invariant_t (t t': Type) = {
+  s: Seq.seq t;
+  l1: list t';
+  r: byte_array;
+  vr: v parse_list_kind (list t');
+  n: SZ.t;
+  n': nat;
+}
+
+[@@__reduce__]
+let read_array_payload_invariant0
+  (#t #t': Type)
+  (#k: parser_kind)
+  (p: parser k t')
+  (item_match: t -> t' -> vprop)
+  (n0: SZ.t)
+  (vl0: v parse_list_kind (list t'))
+  (l0: byte_array)
+  (a0: A.array t)
+  (pn: R.ref SZ.t)
+  (pr: R.ref byte_array)
+  (cont: bool)
+: Tot vprop
+= exists_ (fun w ->
+    read_array_payload_invariant_body0 p item_match n0 vl0 l0 a0 pn pr w.s w.l1 w.r w.vr w.n w.n' `star`
+    pure (read_array_payload_invariant_prop k n0 vl0 cont w.s w.l1 w.vr w.n w.n')
+  )
+
+let read_array_payload_invariant
+  (#t #t': Type)
+  (#k: parser_kind)
+  (p: parser k t')
+  (item_match: t -> t' -> vprop)
+  (n0: SZ.t)
+  (vl0: v parse_list_kind (list t'))
+  (l0: byte_array)
+  (a0: A.array t)
+  (pn: R.ref SZ.t)
+  (pr: R.ref byte_array)
+  (cont: bool)
+: Tot vprop
+= read_array_payload_invariant0 p item_match n0 vl0 l0 a0 pn pr cont
+
+let intro_read_array_payload_invariant
+  (#t #t': Type)
+  (#opened: _)
+  (#k: parser_kind)
+  (p: parser k t')
+  (item_match: t -> t' -> vprop)
+  (n0: SZ.t)
+  (vl0: v parse_list_kind (list t'))
+  (l0: byte_array)
+  (a0: A.array t)
+  (pn: R.ref SZ.t)
+  (pr: R.ref byte_array)
+  (l1: list t')
+  (cont: bool)
+  (s: Seq.seq t)
+  (r: byte_array)
+  (vr: v parse_list_kind (list t'))
+  (n: SZ.t)
+  (n': nat)
+: STGhost unit opened
+    (read_array_payload_invariant_body0 p item_match n0 vl0 l0 a0 pn pr s l1 r vr n n')
+    (fun _ -> read_array_payload_invariant p item_match n0 vl0 l0 a0 pn pr cont)
+    (read_array_payload_invariant_prop0 k n0 vl0 cont s l1 vr n n')
+    (fun _ -> True)
+= let w : read_array_payload_invariant_t t t' = {
+    s = s;
+    l1 = l1;
+    r = r;
+    vr = vr;
+    n = n;
+    n' = n';
+  }
+  in
+  rewrite
+    (read_array_payload_invariant_body0 p item_match n0 vl0 l0 a0 pn pr s l1 r vr n n')
+    (read_array_payload_invariant_body0 p item_match n0 vl0 l0 a0 pn pr w.s w.l1 w.r w.vr w.n w.n');
+  rewrite
+    (read_array_payload_invariant0 p item_match n0 vl0 l0 a0 pn pr cont)  
+    (read_array_payload_invariant p item_match n0 vl0 l0 a0 pn pr cont)  
+
+let elim_read_array_payload_invariant
+  (#t #t': Type)
+  (#opened: _)
+  (#k: parser_kind)
+  (p: parser k t')
+  (item_match: t -> t' -> vprop)
+  (n0: SZ.t)
+  (vl0: v parse_list_kind (list t'))
+  (l0: byte_array)
+  (a0: A.array t)
+  (pn: R.ref SZ.t)
+  (pr: R.ref byte_array)
+  (cont: bool)
+: STGhost (read_array_payload_invariant_t t t') opened
+    (read_array_payload_invariant p item_match n0 vl0 l0 a0 pn pr cont)
+    (fun w -> read_array_payload_invariant_body0 p item_match n0 vl0 l0 a0 pn pr w.s w.l1 w.r w.vr w.n w.n')
+    True
+    (fun w -> read_array_payload_invariant_prop k n0 vl0 cont w.s w.l1 w.vr w.n w.n')
+= rewrite
+    (read_array_payload_invariant p item_match n0 vl0 l0 a0 pn pr cont)
+    (read_array_payload_invariant0 p item_match n0 vl0 l0 a0 pn pr cont);
+  let _ = gen_elim () in
+  vpattern_replace (fun w -> read_array_payload_invariant_body0 p item_match n0 vl0 l0 a0 pn pr w.s w.l1 w.r w.vr w.n w.n')
+
+let list_append_length_lt
+  (#t: Type)
+  (l0: list t)
+  (n0: SZ.t)
+  (sq0': squash (SZ.v n0 == List.Tot.length l0))
+  (l1: list t)
+  (n: SZ.t)
+  (sq1': squash (SZ.v n == List.Tot.length l1))
+  (l2: list t)
+  (sq0: squash (l1 `List.Tot.append` l2 == l0))
+  (sq1: squash (SZ.v n < SZ.v n0))
+: Tot (squash (Cons? l2))
+= List.Tot.append_length l1 l2
+
+let implies_trans_l1
+  (#opened: _)
+  (p q1 q2 r: vprop)
+: STGhostT unit opened
+    ((p @==> q1) `star` ((q1 `star` q2) @==> r))
+    (fun _ -> (p `star` q2) @==> r)
+= implies_reg_r p q1 q2;
+  implies_trans (p `star` q2) (q1 `star` q2) r
+
+let implies_trans_r1
+  (#opened: _)
+  (q1 p q2 r: vprop)
+: STGhostT unit opened
+    ((p @==> q2) `star` ((q1 `star` q2) @==> r))
+    (fun _ -> (q1 `star` p) @==> r)
+= implies_reg_l q1 p q2;
+  implies_trans (q1 `star` p) (q1 `star` q2) r
+
+let implies_trans_cut
+  (#opened: _)
+  (p q1 q2 r2 r3: vprop)
+: STGhostT unit opened
+    ((p @==> (q1 `star` q2)) `star` ((q2 `star` r2) @==> r3))
+    (fun _ -> (p `star` r2) @==> (q1 `star` r3))
+= implies_reg_l q1 (q2 `star` r2) r3;
+  implies_with_tactic ((q1 `star` q2) `star` r2) (q1 `star` (q2 `star` r2));
+  implies_trans ((q1 `star` q2) `star` r2) (q1 `star` (q2 `star` r2)) (q1 `star` r3);
+  implies_trans_l1 p (q1 `star` q2) r2 (q1 `star` r3)
+
+#push-options "--split_queries always --z3cliopt smt.arith.nl=false --z3rlimit 64"
+#restart-solver
+
+inline_for_extraction noextract let
+read_array_payload_body
+  (#t: Type0)
+  (#t': Type0)
+  (#k: Ghost.erased parser_kind)
+  (#p: parser k t')
+  (j: jumper p)
+  (item_match: t -> t' -> vprop)
+  (read: (
+    (#va: v k t') ->
+    (a: byte_array) ->
+    (alen: SZ.t) ->
+    ST t
+    (aparse p a va)
+    (fun c' ->
+      item_match c' va.contents `star`
+      (item_match c' va.contents `implies_` aparse p a va)
+    )
+    (alen == AP.len (array_of va))
+    (fun _ -> True)
+  ))
+  (n0: SZ.t)
+  (vl0: v parse_list_kind (list t'))
+  (l0: byte_array)
+  (a0: A.array t)
+  (pn: R.ref SZ.t)
+  (pr: R.ref byte_array)
+  (_: unit)
+: STT unit
+    (read_array_payload_invariant p item_match n0 vl0 l0 a0 pn pr true)
+    (fun _ -> exists_ (read_array_payload_invariant p item_match n0 vl0 l0 a0 pn pr))
+= let w = elim_read_array_payload_invariant p item_match n0 vl0 l0 a0 pn pr true in // +6
+  A.pts_to_length a0 _;
+  let vr_cons: squash (Cons? w.vr.contents) = list_append_length_lt vl0.contents n0 () w.l1 w.n () w.vr.contents () () in
+  let r = R.read pr in
+  vpattern_rewrite_with_implies (fun r -> aparse (parse_list p) r _) r; // +5
+  let gr' = ghost_elim_cons_with_implies p r in // +4.2
+  let _ = gen_elim () in
+  let sz = get_parsed_size j r in
+  let r' = hop_aparse_aparse_with_size_with_implies p (parse_list p) r sz gr' in // +4.1
+  implies_trans_r1 // +4 -4.1 -4.2
+    (aparse p r _) // q1
+    (aparse (parse_list p) r' _) // p
+    (aparse (parse_list p) gr' _) // q2
+    (aparse (parse_list p) r _); // r
+  let v1 = vpattern (aparse p r) in
+  let vr' = vpattern (aparse (parse_list p) r') in
+  List.Tot.append_assoc w.l1 [v1.contents] vr'.contents;
+  List.Tot.append_length w.l1 [v1.contents];
+  list_index_append_cons w.l1 v1.contents vr'.contents;
+  let l1' : Ghost.erased (list t') = Ghost.hide (w.l1 `List.Tot.append` [v1.contents]) in
+  R.write pr r';
+  let n = R.read pn in
+  let _ : squash (SZ.v n < Seq.length w.s) = () in
+  let n' = n `SZ.add` 1sz in
+  let n'_as_nat : Ghost.erased nat = SZ.v n' in
+  R.write pn n';
+  let c = read r sz in // +3
+  A.upd a0 n c;
+  let s' = vpattern_replace_erased (A.pts_to a0 full_perm) in
+  seq_seq_match_weaken_with_implies // +2
+    item_match w.s s' (Seq.seq_of_list vl0.contents) (Seq.seq_of_list vl0.contents) 0 w.n';
+  rewrite_with_implies // +1
+    (item_match c _)
+    (seq_seq_match_item item_match s' (Seq.seq_of_list vl0.contents) (SZ.v n));
+  on_range_snoc_with_implies // +0
+    (seq_seq_match_item item_match s' (Seq.seq_of_list vl0.contents))
+    _ _ (SZ.v n) n'_as_nat;
+  (* BEGIN FIXME: this should be automated away *)
+  implies_trans_r2 // -0 -1
+    (seq_seq_match item_match s' (Seq.seq_of_list vl0.contents) 0 n'_as_nat)
+    (seq_seq_match item_match _ _ _ _)
+    (seq_seq_match_item item_match _ _ _)
+    (item_match c _);
+  implies_trans_l2 // -2
+    (seq_seq_match item_match s' (Seq.seq_of_list vl0.contents) 0 n'_as_nat)
+    (seq_seq_match item_match _ _ _ _)
+    (item_match c _)
+    (seq_seq_match item_match _ _ _ _);
+  implies_trans_r2 // -3
+    (seq_seq_match item_match s' (Seq.seq_of_list vl0.contents) 0 n'_as_nat)
+    (seq_seq_match item_match _ _ _ _)
+    (item_match c _)
+    (aparse p _ _);
+  implies_trans_cut // -4
+    (seq_seq_match item_match s' (Seq.seq_of_list vl0.contents) 0 n'_as_nat) // p
+    (seq_seq_match item_match _ _ _ _) // q1
+    (aparse p _ _) // q2
+    (aparse (parse_list p) _ _) // r2
+    (aparse (parse_list p) _ _); // r3
+  implies_trans_r2 // -5
+    (seq_seq_match item_match s' (Seq.seq_of_list vl0.contents) 0 n'_as_nat `star` aparse (parse_list p) _ _)
+    (seq_seq_match item_match _ _ _ _)
+    (aparse (parse_list p) _ _)
+    (aparse (parse_list p) _ _);
+  implies_trans // -6
+    (seq_seq_match item_match s' (Seq.seq_of_list vl0.contents) 0 n'_as_nat `star` aparse (parse_list p) _ _)
+    (seq_seq_match item_match _ _ _ _ `star` aparse (parse_list p) _ _)
+    (aparse (parse_list p) _ _);
+  (* END FIXME *)
+  intro_read_array_payload_invariant p item_match n0 vl0 l0 a0 pn pr l1' (n' `SZ.lt` n0) _ _ _ _ _;
+  return ()
+
+#pop-options
+
+inline_for_extraction
+let read_array_payload_from_list
+  (#t #t': Type)
+  (#k: Ghost.erased parser_kind)
+  (#p: parser k t')
+  (j: jumper p)
+  (item_match: t -> t' -> vprop)
+  (read: (
+    (#va: v k t') ->
+    (a: byte_array) ->
+    (alen: SZ.t) ->
+    ST t
+    (aparse p a va)
+    (fun c' ->
+      item_match c' va.contents `star`
+      (item_match c' va.contents `implies_` aparse p a va)
+    )
+    (alen == AP.len (array_of va))
+    (fun _ -> True)
+  ))
+  (n0: SZ.t)
+  (#vl0: v parse_list_kind (list t'))
+  (l0: byte_array)
+  (#va0: Ghost.erased (Seq.seq t))
+  (a0: A.array t)
+: ST (Ghost.erased (Seq.seq t))
+    (A.pts_to a0 full_perm va0 `star`
+      aparse (parse_list p) l0 vl0
+    )
+    (fun res ->
+      A.pts_to a0 full_perm res `star`
+      seq_list_match res vl0.contents item_match `star`
+      (seq_list_match res vl0.contents item_match `implies_`
+        aparse (parse_list p) l0 vl0
+      )
+    )
+    (A.length a0 == SZ.v n0 /\
+      List.Tot.length vl0.contents == SZ.v n0 /\
+      k.parser_kind_subkind == Some ParserStrong
+    )
+    (fun _ -> True)
+= A.pts_to_length a0 _;
+  on_range_empty
+    (seq_seq_match_item item_match va0 (Seq.seq_of_list vl0.contents))
+    0 0;
+  intro_implies
+    (seq_seq_match item_match va0 (Seq.seq_of_list vl0.contents) 0 0 `star`
+      aparse (parse_list p) l0 vl0)
+    (aparse (parse_list p) l0 vl0)
+    emp
+    (fun _ -> drop (seq_seq_match item_match _ _ _ _));
+  R.with_local 0sz (fun pn ->
+  R.with_local l0 (fun pr ->
+    intro_read_array_payload_invariant p item_match n0 vl0 l0 a0 pn pr [] (0sz `SZ.lt` n0) _ _ _ _ _;
+    Steel.ST.Loops.while_loop
+      (read_array_payload_invariant p item_match n0 vl0 l0 a0 pn pr)
+      (fun _ ->
+        let gcont = elim_exists () in
+        let w = elim_read_array_payload_invariant p item_match n0 vl0 l0 a0 pn pr gcont in
+        let n = R.read pn in
+        [@@inline_let]
+        let cont = n `SZ.lt` n0 in
+        intro_read_array_payload_invariant p item_match n0 vl0 l0 a0 pn pr w.l1 cont _ _ _ _ _;
+        return cont
+      )
+      (read_array_payload_body j item_match read n0 vl0 l0 a0 pn pr);
+    let w = elim_read_array_payload_invariant p item_match n0 vl0 l0 a0 pn pr false in
+    List.Tot.append_length w.l1 w.vr.contents;
+    assert (Nil? w.vr.contents);
+    List.Tot.append_l_nil w.l1;
+    A.pts_to_length a0 _;
+    rewrite_with_implies
+      (seq_seq_match item_match _ _ _ _)
+      (seq_seq_match item_match w.s (Seq.seq_of_list vl0.contents) 0 (List.Tot.length vl0.contents));
+    seq_seq_match_seq_list_match_with_implies item_match _ vl0.contents;
+    implies_trans
+      (seq_list_match w.s vl0.contents item_match)
+      (seq_seq_match item_match _ _ _ _)
+      (seq_seq_match item_match _ _ _ _);
+    implies_concl_r
+      (seq_list_match w.s vl0.contents item_match)
+      (seq_seq_match item_match _ _ _ _)
+      (aparse (parse_list p) _ _);
+    implies_trans
+      (seq_list_match w.s vl0.contents item_match)
+      (seq_seq_match item_match _ _ _ _ `star` aparse (parse_list p) _ _)
+      (aparse (parse_list p) _ _);
+    return (Ghost.hide w.s)
+  ))
+
+inline_for_extraction
+let read_array_payload_from_nlist
+  (#t #t': Type)
+  (#k: Ghost.erased parser_kind)
+  (#p: parser k t')
+  (j: jumper p)
+  (item_match: t -> t' -> vprop)
+  (read: (
+    (#va: v k t') ->
+    (a: byte_array) ->
+    (alen: SZ.t) ->
+    ST t
+    (aparse p a va)
+    (fun c' ->
+      item_match c' va.contents `star`
+      (item_match c' va.contents `implies_` aparse p a va)
+    )
+    (alen == AP.len (array_of va))
+    (fun _ -> True)
+  ))
+  (n0: SZ.t)
+  (#vl0: v (parse_nlist_kind (SZ.v n0) k) (nlist (SZ.v n0) t'))
+  (l0: byte_array)
+  (#va0: Ghost.erased (Seq.seq t))
+  (a0: A.array t)
+: ST (Ghost.erased (Seq.seq t))
+    (A.pts_to a0 full_perm va0 `star`
+      aparse (parse_nlist (SZ.v n0) p) l0 vl0
+    )
+    (fun res ->
+      A.pts_to a0 full_perm res `star`
+      seq_list_match res vl0.contents item_match `star`
+      (seq_list_match res vl0.contents item_match `implies_`
+        aparse (parse_nlist (SZ.v n0) p) l0 vl0
+      )
+    )
+    (A.length a0 == SZ.v n0 /\
+      k.parser_kind_low > 0 /\
+      k.parser_kind_subkind == Some ParserStrong
+    )
+    (fun _ -> True)
+= A.pts_to_length a0 _;
+  let vl = aparse_nlist_aparse_list_with_implies p (SZ.v n0) l0 in
+  let res = read_array_payload_from_list j item_match read n0 l0 a0 in
+  rewrite_with_implies
+    (seq_list_match _ vl.contents item_match)
+    (seq_list_match _ vl0.contents item_match);
+  implies_trans
+    (seq_list_match _ _ item_match)
+    (seq_list_match _ _ item_match)
+    (aparse (parse_list p) _ _);
+  implies_trans
+    (seq_list_match _ _ item_match)
+    (aparse (parse_list p) _ _)
+    (aparse (parse_nlist (SZ.v n0) p) _ _);
+  return res
